\documentclass{article}
\usepackage[utf8]{inputenc}
\usepackage[english]{babel}
\usepackage{amsmath}
\usepackage[]{amsthm} %lets us use \begin{proof}
\usepackage[]{amssymb} %gives us the character \varnothing

\title{DATA 558: Homework 1}
\author{Trevor Nims}
\date\today


\begin{document}
\maketitle

\section*{Exercise 1}
In this section, I will compute the derivatives of the following functions with respect to the parameter $\beta \in \mathbb{R}$.
\\\\
\indent 1. $f(\beta) = \frac{1}{2n}\sum_{i=1}^{n}(y_1-x_i\beta)^2$

\begin{align*}
	\frac{d}{d\beta}f(\beta) &= -\frac{2}{2n}\sum_{i=1}^{n} x_i(y_i-x_i\beta) \\
	&= -\frac{1}{2n}\sum_{i=1}^{n} x_iy_i-x_i^2\beta
\end{align*}
\\\\
\indent 2. $f(\beta) = \frac{e^{x\beta}}{e^{x\beta}+1}$
\begin{align*}
	\frac{d}{d\beta}f(\beta) &=	\frac{d}{d\beta}\bigg(e^{x\beta}(e^{x\beta}+1)^{-1}\bigg) \\
	&= \frac{xe^{x\beta}}{e^{x\beta}+1}-\frac{e^{x\beta}xe^{x\beta}}{(e^{x\beta}+1)^2} \\
	&= \frac{xe^{x\beta}}{e^{x\beta}+1}-\frac{xe^{2x\beta}}{(e^{x\beta}+1)^2} 
\end{align*}
\\\\
\indent 3. $f(\beta) = \text{log}(\sum_{i=1}^{n}e^{x_i\beta-1})$
\begin{align*}
	\frac{d}{d\beta}f(\beta) &= \frac{1}{\sum_{i=1}^{n}e^{x_i\beta-1}}\cdot\sum_{i=1}^{n}x_ie^{x_i\beta-1} \\
	&= \sum_{i=1}^{n}x_i
\end{align*}
\\\\
\indent 4. $f(\beta) = |y-x\beta|$
\\
\[f(\beta) =  \begin{cases}
	y-x\beta & \beta \leq \frac{y}{x} \\
	-(y-x\beta) & \beta > \frac{y}{x}
\end{cases}
\] \\

\[ \frac{d}{d\beta}f(\beta) =  \begin{cases}
	-x & \beta \leq \frac{y}{x} \\
	x & \beta > \frac{y}{x}
\end{cases}
\] \\

\end{document}